update remaining rules, split mutex into lib

theories/logrel/term_types.v
@@ -7,7 +7,7 @@ From actris.channel Require Export channel.
 Definition lty_any {Σ} : ltty Σ := Ltty (λ w, True%I).
 
 Definition lty_copy {Σ} (A : ltty Σ) : ltty Σ := Ltty (λ w, □ ltty_car A w)%I.
-Definition lty_copy_inv {Σ} (A : ltty Σ) : ltty Σ := Ltty (λ w, coreP (ltty_car A w)).
+Definition lty_copy_minus {Σ} (A : ltty Σ) : ltty Σ := Ltty (λ w, coreP (ltty_car A w)).
 Definition lty_copyable {Σ} (A : ltty Σ) : iProp Σ :=
   tc_opaque (A <: lty_copy A)%I.
 
@@ -35,21 +35,11 @@ Definition ref_shrN := nroot .@ "shr_ref".
 Definition lty_ref_shr `{heapG Σ} (A : ltty Σ) : ltty Σ := Ltty (λ w,
   ∃ l : loc, ⌜w = #l⌝ ∗ inv (ref_shrN .@ l) (∃ v, l ↦ v ∗ ltty_car A v))%I.
 
-Definition lty_mutex `{heapG Σ, lockG Σ} (A : ltty Σ) : ltty Σ := Ltty (λ w,
-  ∃ (γ : gname) (l : loc) (lk : val),
-    ⌜ w = PairV lk #l ⌝ ∗
-    is_lock γ lk (∃ v_inner, l ↦ v_inner ∗ ltty_car A v_inner))%I.
-Definition lty_mutexguard `{heapG Σ, lockG Σ} (A : ltty Σ) : ltty Σ := Ltty (λ w,
-  ∃ (γ : gname) (l : loc) (lk : val) (v : val),
-    ⌜ w = PairV lk #l ⌝ ∗
-    is_lock γ lk (∃ v_inner, l ↦ v_inner ∗ ltty_car A v_inner) ∗
-    spin_lock.locked γ ∗ l ↦ v)%I.
-
 Definition lty_chan `{heapG Σ, chanG Σ} (P : lsty Σ) : ltty Σ :=
   Ltty (λ w, w ↣ lsty_car P)%I.
 
 Instance: Params (@lty_copy) 1 := {}.
-Instance: Params (@lty_copy_inv) 1 := {}.
+Instance: Params (@lty_copy_minus) 1 := {}.
 Instance: Params (@lty_copyable) 1 := {}.
 Instance: Params (@lty_arr) 2 := {}.
 Instance: Params (@lty_prod) 1 := {}.
@@ -58,14 +48,12 @@ Instance: Params (@lty_forall) 2 := {}.
 Instance: Params (@lty_sum) 1 := {}.
 Instance: Params (@lty_ref_mut) 2 := {}.
 Instance: Params (@lty_ref_shr) 2 := {}.
-Instance: Params (@lty_mutex) 3 := {}.
-Instance: Params (@lty_mutexguard) 3 := {}.
 Instance: Params (@lty_chan) 3 := {}.
 
 Notation any := lty_any.
 Notation "()" := lty_unit : lty_scope.
 Notation "'copy' A" := (lty_copy A) (at level 10) : lty_scope.
-Notation "'copy-' A" := (lty_copy_inv A) (at level 10) : lty_scope.
+Notation "'copy-' A" := (lty_copy_minus A) (at level 10) : lty_scope.
 
 Notation "A ⊸ B" := (lty_arr A B)
   (at level 99, B at level 200, right associativity) : lty_scope.
@@ -81,9 +69,6 @@ Notation "∃ A1 .. An , C" :=
 Notation "'ref_mut' A" := (lty_ref_mut A) (at level 10) : lty_scope.
 Notation "'ref_shr' A" := (lty_ref_shr A) (at level 10) : lty_scope.
 
-Notation "'mutex' A" := (lty_mutex A) (at level 10) : lty_scope.
-Notation "'mutexguard' A" := (lty_mutexguard A) (at level 10) : lty_scope.
-
 Notation "'chan' A" := (lty_chan A) (at level 10) : lty_scope.
 
 Section term_types.
@@ -92,7 +77,7 @@ Section term_types.
 
   Global Instance lty_copy_ne : NonExpansive (@lty_copy Σ).
   Proof. solve_proper. Qed.
-  Global Instance lty_copy_inv_ne : NonExpansive (@lty_copy_inv Σ).
+  Global Instance lty_copy_minus_ne : NonExpansive (@lty_copy_minus Σ).
   Proof. solve_proper. Qed.
 
   Global Instance lty_copyable_plain A : Plain (lty_copyable A).
@@ -142,17 +127,6 @@ Section term_types.
   Global Instance lty_ref_shr_contractive `{heapG Σ} : Contractive lty_ref_shr.
   Proof. solve_contractive. Qed.
   Global Instance lty_ref_shr_ne `{heapG Σ} : NonExpansive lty_ref_shr.
-  Proof. solve_proper. Qed.
-
-  Global Instance lty_mutex_contractive `{heapG Σ, lockG Σ} : Contractive lty_mutex.
-  Proof. solve_contractive. Qed.
-  Global Instance lty_mutex_ne `{heapG Σ, lockG Σ} : NonExpansive lty_mutex.
-  Proof. solve_proper. Qed.
-
-  Global Instance lty_mutexguard_contractive `{heapG Σ, lockG Σ} :
-    Contractive lty_mutexguard.
-  Proof. solve_contractive. Qed.
-  Global Instance lty_mutexguard_ne `{heapG Σ, lockG Σ} : NonExpansive lty_mutexguard.
   Proof. solve_proper. Qed.
 
   Global Instance lty_chan_ne `{heapG Σ, chanG Σ} : NonExpansive lty_chan.
